Implementation of mapping db functions
Todo: Proofs

AssocList.v
@@ -31,69 +31,67 @@ Fixpoint assoc (k:N) (l:assoc_list) : option T :=
   end.
 Global Arguments assoc : default implicits.
 
-Fixpoint rev_assoc (p:T -> bool) (l:assoc_list) : list N :=
-  match l with
-    | nil         => nil
-    | (k,v) :: t => if p v then k :: rev_assoc p t else rev_assoc p t
-  end.
-Global Arguments rev_assoc : default implicits.
-
-Fixpoint merge (f:T -> T -> T) (l1:assoc_list) (l2:assoc_list) : assoc_list :=
-  match l1 with
-    | nil        => l2
-    | (k,v1) :: l1_t =>
-      match assoc k l2 with
-        | None    => (k,v1) :: merge f l1_t l2
-        | Some v2 => (k,f v1 v2) :: merge f l1_t (remove k l2)
-      end
-  end.
-Global Arguments merge : default implicits.
-
-Definition union : assoc_list -> assoc_list -> assoc_list :=
-  merge (fun _ b => b).
-Global Arguments union : default implicits.
-
-Fixpoint fold {X:Type} (f:N -> T -> X -> X) (x:X) (l:assoc_list) : X :=
-  match l with
-    | nil        => x
-    | (k,v) :: t => f k v (fold f x t)
-  end.
-Global Arguments fold : default implicits.
-
 End AssocListDef.
-
 
 Section InvariantDef.
 
 Variable T : Type.
 
-Definition in_domain (k:N) (l:assoc_list T) : Prop :=
-  exists v, In (k,v) l.
+Definition contains (k:N) (P:T -> Prop) (l:assoc_list T) : Prop :=
+  exists v, In (k,v) l /\ P v.
+
+Lemma contains_inv :
+  forall (k:N) (P:T -> Prop) (k':N) (v:T) (l:assoc_list T),
+    contains k P ((k',v) :: l) <-> (k' = k /\ P v) \/ contains k P l.
+Proof.
+  Hint Resolve in_eq in_cons.
+  intros k P k' v l. unfold contains. split.
+  - destruct 1 as [v' [in_k HP]]. apply in_inv in in_k. destruct in_k.
+    + inversion H. subst. tauto.
+    + eauto.
+  - destruct 1 as [[ke HP]|[v' [v'_in HP]]]; subst; intuition eauto.
+Qed.
+
+Lemma contains_app_or :
+  forall (k:N) (P:T -> Prop) (l1 l2:assoc_list T),
+    contains k P (l1 ++ l2) <-> contains k P l1 \/ contains k P l2.
+Proof.
+  Hint Resolve in_or_app .
+  unfold contains.
+  intros k P l1 l2. split.
+  - destruct 1 as [v [in_l12 HP]]. apply in_app_or in in_l12. intuition eauto.
+  - destruct 1 as [in_l|in_l]; destruct in_l as [v [in_l HP]]; eauto.
+Qed.
+
+Definition in_domain (k:N) : assoc_list T -> Prop := contains k (fun _ => True).
+
+Theorem contains_in_domain :
+  forall (l:assoc_list T) (k:N) (P:T -> Prop), contains k P l -> in_domain k l.
+Proof.
+  unfold in_domain. unfold contains. intros l k P. destruct 1. intuition eauto.
+Qed.
 
 Lemma in_domain_inv :
   forall (k:N) (k':N) (v:T) (l:assoc_list T),
     in_domain k ((k',v) :: l) <-> k' = k \/ in_domain k l.
+Proof. unfold in_domain. intros. rewrite contains_inv. tauto. Qed.
+
+Theorem in_domain_contains_eq :
+  forall (l:assoc_list T) (k:N), in_domain k l -> exists v, contains k (eq v) l.
 Proof.
-  intros k k' v l. split.
-  - intros H. unfold in_domain in H. destruct H as [v' k_in].
-    apply in_inv in k_in. destruct k_in.
-    + inversion H. subst. tauto.
-    + unfold in_domain. eauto.
-  - unfold in_domain. intros H. destruct H as [H|H].
-    + subst. exists v. apply in_eq.
-    + destruct H as [v' v'_in]. exists v'. apply in_cons. assumption.
+  Hint Resolve in_domain_inv in_nil.
+  intros l k. induction l as [|[k' v] t IH].
+  - destruct 1. exfalso. intuition auto.
+  - unfold in_domain. unfold contains. destruct 1 as [v' [k_in _]].
+    apply in_inv in k_in. case k_in.
+    + inversion 1. subst. eauto.
+    + eauto.
 Qed.
 
 Lemma in_domain_app_or :
   forall (k:N) (l1 l2:assoc_list T),
     in_domain k (l1 ++ l2) <-> in_domain k l1 \/ in_domain k l2.
-Proof.
-  Hint Resolve in_or_app.
-  Hint Unfold in_domain.
-  intros k l1 l2. split.
-  - destruct 1 as [v in_l12]. apply in_app_or in in_l12. intuition eauto.
-  - destruct 1 as [in_l | in_l]; destruct in_l as [v in_l]; intuition eauto.
-Qed.
+Proof. unfold in_domain. intros. rewrite contains_app_or. tauto. Qed.
 
 Definition al_disjoint (l1 l2:assoc_list T) : Prop :=
   forall k, in_domain k l1 -> ~in_domain k l2.
@@ -101,24 +99,13 @@ Definition al_disjoint (l1 l2:assoc_list T) : Prop :=
 Lemma al_disjoint_nil_l :
   forall (l1:assoc_list T), al_disjoint nil l1.
 Proof.
-  intros l1. unfold al_disjoint. unfold in_domain. intros k in_nil.
-  destruct in_nil as [v v_in_nil]. inversion v_in_nil.
+  intros l1 k. unfold in_domain. unfold contains. destruct 1 as [v [in_nil HP]].
+  contradiction.
 Qed.
 
 Lemma al_disjoint_symmetry :
   forall (l1 l2:assoc_list T), al_disjoint l1 l2 -> al_disjoint l2 l1.
-Proof.
-  unfold al_disjoint. unfold in_domain. unfold not.
-  intuition eauto.
-Qed.
-
-Lemma al_disjoint_app_split :
-  forall (l1 l2 l3:assoc_list T),
-    al_disjoint (l1 ++ l2) l3 -> al_disjoint l1 l3 /\ al_disjoint l2 l3.
-Proof.
-  Hint Resolve <- in_domain_app_or.
-  unfold al_disjoint. intros l1 l2 l3 H. split; intros k P; apply H; eauto.
-Qed.
+Proof. unfold al_disjoint. eauto. Qed.
 
 Lemma al_disjoint_cons_not_elem :
   forall (l1 l2:assoc_list T) (k:N) (v:T),
@@ -154,12 +141,12 @@ Lemma al_invariant_app_split :
     al_invariant (l1 ++ l2) -> al_invariant l1 /\ al_invariant l2.
 Proof.
   Hint Constructors al_invariant.
-  Hint Resolve in_domain_app_or al_invariant_cons.
+  Hint Resolve <- in_domain_app_or.
   intros l1 l2 H. induction l1 as [|h t IH].
   - auto.
   - destruct h as [k v]. inversion H as [|k' v' t' not_in_tl2 inv_tl2]; subst. split;
       try (apply al_invariant_cons);
-      intuition auto.
+      intuition eauto.
 Qed.
 
 Lemma al_invariant_join_app :
@@ -185,6 +172,36 @@ Proof.
   - apply al_invariant_disjoint in H. apply al_disjoint_symmetry. apply H.
 Qed.
 
+Lemma al_invariant_in_eq :
+  forall (l:assoc_list T) (k:N) (v v':T),
+    al_invariant l -> In (k,v) l -> In (k,v') l -> v = v'.
+Proof.
+  Hint Resolve in_inv contains_in_domain.
+  Hint Unfold contains in_domain not.
+  intros l k v v' inv_l v_in v'_in. induction l as [|[k' v''] t IH].
+  - destruct v_in.
+  - inversion inv_l. subst. case v_in.
+    + inversion 1. subst. case v'_in.
+      * inversion 1. auto.
+      * intros. exfalso. eauto 6.
+    + intros. case v'_in.
+      * inversion 1. subst. exfalso. eauto 6.
+      * auto.
+Qed.
+
+Lemma contains_combine :
+  forall (l:assoc_list T) (k:N) (P1 P2:T -> Prop),
+    al_invariant l -> contains k P1 l -> contains k P2 l ->
+    contains k (fun x => P1 x /\ P2 x) l.
+Proof.
+  Hint Resolve al_invariant_in_eq.
+  unfold contains.
+  intros l k P1 P2 inv_l c_P1 c_P2.
+  destruct c_P1 as [v [in1 HP1]].
+  destruct c_P2 as [v' [in2 HP2]].
+  assert (eq: v' = v); subst; eauto.
+Qed.
+
 End InvariantDef.
 
 
@@ -205,33 +222,35 @@ Section RemoveTheorems.
 Variable T : Type.
 
 Theorem remove_subset :
-  forall (l:assoc_list T) (k k':N), in_domain T k (remove k' l) -> in_domain T k l.
+  forall (l:assoc_list T) (k k':N) (P:T -> Prop),
+    contains T k P (remove k' l) -> contains T k P l.
 Proof.
-  Hint Resolve <- in_domain_inv.
-  intros l k k'. induction l as [|[k'' v] t IH].
-  - destruct 1. contradiction.
+  Hint Resolve <- contains_inv.
+  intros l k k' P. induction l as [|[k'' v] t IH].
+  - destruct 1 as [v [in_nil HP]]. contradiction.
   - simpl. destruct (N.eq_dec k'' k').
     + auto.
-    + rewrite in_domain_inv. destruct 1; subst; auto.
+    + rewrite contains_inv. destruct 1; subst; auto.
 Qed.
 
 Theorem remove_invariant :
   forall (l:assoc_list T) (k:N), al_invariant T l -> al_invariant T (remove k l).
 Proof.
-  Hint Unfold not.
+  Hint Unfold not in_domain.
   Hint Resolve remove_subset al_invariant_cons.
   intros l k. induction l as [|[k' v] t IH].
   - trivial.
-  - inversion 1. subst. simpl. destruct (N.eq_dec k' k); intuition eauto.
+  - inversion 1. subst. simpl.
+    destruct (N.eq_dec k' k); intuition eauto 6.
 Qed.
 
 Theorem remove_preserve_other :
-  forall (l:assoc_list T) (k k':N),
-    k' <> k -> in_domain T k l -> in_domain T k (remove k' l).
+  forall (l:assoc_list T) (k k':N) (P:T -> Prop),
+    k' <> k -> contains T k P l -> contains T k P (remove k' l).
 Proof.
-  intros l k k' ineq. induction l as [|[k'' v] t IH].
-  - destruct 1. contradiction.
-  - simpl. rewrite in_domain_inv. destruct (N.eq_dec k'' k').
+  intros l k k' P ineq. induction l as [|[k'' v] t IH].
+  - trivial.
+  - simpl. rewrite contains_inv. destruct (N.eq_dec k'' k').
     + subst. tauto.
     + intuition auto.
 Qed.
@@ -240,7 +259,7 @@ Theorem not_in_remove :
   forall (l:assoc_list T) (k:N), al_invariant T l -> ~in_domain T k (remove k l).
 Proof.
   intros l k inv_l. induction l as [|[k' v] t IH].
-  - destruct 1. contradiction.
+  - destruct 1. intuition auto.
   - simpl. inversion inv_l. subst. destruct (N.eq_dec k' k); subst.
     + auto.
     + rewrite in_domain_inv. tauto.
@@ -252,12 +271,13 @@ Section InsertTheorems.
 
 Variable T : Type.
 
-Theorem insert_superset :
-  forall (l:assoc_list T) (k k':N) (v:T), 
+Theorem insert_domain_superset :
+  forall (l:assoc_list T) (k k':N) (v:T),
     in_domain T k l -> in_domain T k (insert k' v l).
 Proof.
   Hint Resolve <- in_domain_inv.
   Hint Resolve remove_preserve_other.
+  Hint Unfold in_domain.
   intros. unfold insert. destruct (N.eq_dec k k'); auto.
 Qed.
 
@@ -269,16 +289,21 @@ Proof.
 Qed.
 
 Theorem insert_preserve_other :
-  forall (l:assoc_list T) (k k':N) (v:T),
-    k' <> k -> in_domain T k (insert k' v l) -> in_domain T k l.
+  forall (l:assoc_list T) (k k':N) (v:T) (P:T -> Prop),
+    k' <> k -> (contains T k P (insert k' v l) <-> contains T k P l).
 Proof.
   Hint Resolve remove_subset.
-  intros l k k' v ineq.  unfold insert. rewrite in_domain_inv. intuition eauto.
+  intros l k k' v P ineq. unfold insert. rewrite contains_inv. split; intuition eauto.
 Qed.
+
+Theorem contains_insert :
+  forall (l:assoc_list T) (k:N) (v:T) (P:T -> Prop),
+    P v -> contains T k P (insert k v l).
+Proof. intros. unfold insert. apply contains_inv. tauto. Qed.
 
 Theorem in_insert :
   forall (l:assoc_list T) (k:N) (v:T), in_domain T k (insert k v l).
-Proof. intros. unfold insert. apply in_domain_inv. tauto. Qed.
+Proof. intros. apply contains_insert. apply I. Qed.
 
 End InsertTheorems.
 
@@ -286,44 +311,88 @@ Section AssocTheorems.
 
 Variable T : Type.
 
-Theorem assoc_in :
-  forall (l:assoc_list T) (k:N), (exists v, assoc k l = Some v) <-> in_domain T k l.
+Theorem assoc_in_contains :
+  forall (l:assoc_list T) (k:N) (v:T),
+    assoc k l = Some v -> contains T k (eq v) l.
 Proof.
-  Hint Resolve <- in_domain_inv.
-  intros l k. split.
-  - induction l as [|[k' v'] t IH].
-    + destruct 1. discriminate.
-    + simpl. destruct (N.eq_dec k' k); subst; auto.
-  - induction l as [|[k' v'] t IH].
-    + destruct 1. contradiction.
-    + rewrite in_domain_inv. simpl. destruct (N.eq_dec k' k); subst; intuition eauto.
+  Hint Resolve <- contains_inv.
+  intros l k v.
+  induction l as [|[k' v'] t IH].
+    + discriminate.
+    + simpl. destruct (N.eq_dec k' k); inversion 1; subst; auto.
 Qed.
+
+Theorem contains_assoc_in :
+  forall (l:assoc_list T) (k:N) (v:T),
+    al_invariant T l -> contains T k (eq v) l -> assoc k l = Some v.
+Proof.
+  Hint Resolve contains_in_domain.
+  intros l k v inv_l.
+  - induction l as [|[k' v'] t IH].
+    + destruct 1 as [v' [H HP]]. contradiction.
+    + inversion inv_l. subst. rewrite contains_inv. simpl. destruct (N.eq_dec k' k).
+      * destruct 1 as [[ke ve] | contains_in]; [|exfalso]; subst; eauto.
+      * intuition auto.
+Qed.
+
+Theorem assoc_in_domain :
+  forall (l:assoc_list T) (k:N),
+    (exists v, assoc k l = Some v) <-> in_domain T k l.
+Proof.
+   Hint Resolve <- in_domain_inv.
+   intros l k. split.
+   - induction l as [|[k' v'] t IH].
+     + destruct 1. discriminate.
+     + simpl. destruct (N.eq_dec k' k); subst; auto.
+   - induction l as [|[k' v'] t IH].
+     + destruct 1. exfalso. intuition auto.
+     + rewrite in_domain_inv. simpl. destruct (N.eq_dec k' k); subst; intuition eauto.
+Qed.
+
+Theorem assoc_in_1 :
+  forall (l:assoc_list T) (k:N) (v:T),
+    assoc k l = Some v -> in_domain T k l.
+Proof. Hint Resolve -> assoc_in_domain. eauto. Qed.
 
 Theorem assoc_not_in :
   forall (l:assoc_list T) (k:N), assoc k l = None <-> ~in_domain T k l.
 Proof.
+  Hint Resolve assoc_in_contains.
   intros. split.
   - destruct (assoc k l) eqn:A.
     + discriminate 1.
-    + intros. rewrite <- assoc_in. rewrite A. destruct 1. discriminate.
+    + intros. rewrite <- assoc_in_domain. rewrite A. destruct 1. discriminate.
   - destruct (assoc k l) eqn:A.
-    + intros.
-      apply ex_intro with (P := fun x => assoc k l = Some x) in A.
-      apply assoc_in in A. contradiction.
+    + intros. exfalso. eauto.
     + reflexivity.
 Qed.
 
 End AssocTheorems.
 
-Section MergeTheorems.
+Section Merge.
 
 Variable T : Type.
+
+Fixpoint merge (f:T -> T -> T) (l1:assoc_list T) (l2:assoc_list T) : assoc_list T :=
+  match l1 with
+    | nil        => l2
+    | (k,v1) :: l1_t =>
+      match assoc k l2 with
+        | None    => (k,v1) :: merge f l1_t l2
+        | Some v2 => (k,f v1 v2) :: merge f l1_t (remove k l2)
+      end
+  end.
+Global Arguments merge : default implicits.
+
+Definition union : assoc_list T -> assoc_list T -> assoc_list T :=
+  merge (fun _ b => b).
+Global Arguments union : default implicits.
 
 Theorem merge_no_new_elements :
   forall (l1 l2:assoc_list T) (f:T -> T -> T) (k:N),
     ~in_domain T k l1 -> ~in_domain T k l2 -> ~in_domain T k (merge f l1 l2).
 Proof.
-  Hint Unfold not.
+  Hint Unfold not in_domain.
   Hint Resolve remove_subset.
   intros l1 l2 f k H.
   generalize dependent l2.
@@ -338,14 +407,12 @@ Theorem merge_invariant :
     al_invariant T l1 -> al_invariant T l2 -> al_invariant T (merge f l1 l2).
 Proof.
   Hint Resolve al_invariant_cons merge_no_new_elements not_in_remove remove_invariant.
+  Hint Resolve -> assoc_not_in assoc_in_domain.
   intros l1 l2 f inv_l1.
   generalize dependent l2.
   induction l1 as [|[k v] t IH].
   - intros. assumption.
-  - intros l2 inv_l2. inversion inv_l1. subst. simpl. destruct (assoc k l2) eqn:A.
-    + apply ex_intro with (P := fun x => assoc k l2 = Some x) in A.
-      apply assoc_in in A. auto.
-    + apply assoc_not_in in A. auto.
+  - intros l2 inv_l2. inversion inv_l1. subst. simpl. case_eq (assoc k l2); auto.
 Qed.
 
 Theorem merge_superset_first :
@@ -357,8 +424,8 @@ Proof.
   intros l1 l2 f k.
   generalize dependent l2.
   - induction l1 as [|[k' v] t IH].
-    + destruct 1. contradiction.
-    + intros l2. rewrite in_domain_inv. intros H. simpl.
+    + destruct 1. exfalso. intuition auto.
+    + intros l2. rewrite in_domain_inv. simpl.
       destruct (assoc k' l2) eqn:A; intuition auto.
 Qed.
 
@@ -366,39 +433,105 @@ Theorem merge_superset_second :
   forall (l1 l2:assoc_list T) (f:T -> T -> T) (k:N),
     in_domain T k l2 -> in_domain T k (merge f l1 l2).
 Proof.
-  Hint Resolve <- in_domain_inv.
+  Hint Resolve <- contains_inv.
   Hint Resolve remove_preserve_other.
   intros l1 l2 f k.
   generalize dependent l2.
-  - induction l1 as [|[k' v] t IH].
+  - unfold in_domain. induction l1 as [|[k' v] t IH].
     + trivial.
     + intros l2. intros H. simpl.
       destruct (assoc k' l2) eqn:A; destruct (N.eq_dec k' k); subst; auto.
 Qed.
 
-End MergeTheorems.
+End Merge.
 
-Section RevAssocTheorems.
+Section RevAssoc.
 
 Variable T : Type.
+
+Fixpoint rev_assoc (p:T -> bool) (l:assoc_list T) : list N :=
+  match l with
+    | nil         => nil
+    | (k,v) :: t => if p v then k :: rev_assoc p t else rev_assoc p t
+  end.
+Global Arguments rev_assoc : default implicits.
 
 Theorem rev_assoc_assoc :
   forall (f:T -> bool) (l:assoc_list T) (k:N),
     al_invariant T l ->
-    (In k (rev_assoc f l) <-> exists v, assoc k l = Some v /\ f v = true).
+    In k (rev_assoc f l) -> contains T k (fun v => f v = true) l.
 Proof.
-  intros f l k inv_l. split.
-  - generalize dependent k. induction l as [|[k' v'] t IH].
-    + contradiction.
-    + intros k. simpl. destruct (N.eq_dec k' k).
-      * subst. destruct (f v') eqn:fv.
-        intros. exists v'. split; auto.
-        intros H. inversion inv_l. destruct IH with k as [v'' [A FVT]].
-        assumption.
-        assumption.
-        apply ex_intro with (P := fun x => assoc k t = Some x) in A.
-        apply assoc_in in A. contradiction.
-      * destruct (f v') eqn:fv. intros H. apply in_inv in H. inversion inv_l. 
-        intuition eauto.
-        intros H. inversion inv_l. auto.
-Abort.
+  intros f l k inv_l H. induction l as [|[k' v'] t IH].
+  - contradiction.
+  - apply contains_inv. simpl in H. inversion inv_l. subst. destruct (f v') eqn:fv.
+    + apply in_inv in H. destruct (N.eq_dec k' k); intuition eauto.
+    + destruct (N.eq_dec k' k). subst.
+      * Hint Resolve contains_in_domain. exfalso. intuition eauto.
+      * eauto.
+Qed.
+
+Theorem assoc_rev_assoc :
+  forall (f:T -> bool) (l:assoc_list T) (k:N),
+    al_invariant T l ->
+    contains T k (fun v => f v = true) l -> In k (rev_assoc f l).
+Proof.
+  Hint Unfold contains.
+  Hint Resolve in_eq in_cons.
+  intros f l k inv_l. induction l as [|[k' v'] t IH].
+  - destruct 1 as [v [a fv]]. auto.
+  - simpl. inversion inv_l. subst. destruct 1 as [v [v_in fvt]].
+    apply in_inv in v_in. destruct v_in as [eq|in_t].
+    + inversion eq. subst. rewrite fvt. auto.
+    + destruct (f v') eqn:fv'; eauto 6.
+Qed.
+
+End RevAssoc.
+
+Section Filter.
+
+Variable T : Type.
+
+Definition al_filter (f:N -> T -> bool) : assoc_list T -> assoc_list T :=
+  filter (fun x => match x with (k,v) => f k v end).
+Global Arguments al_filter : default implicits.
+
+Theorem al_filter_subset :
+  forall (l:assoc_list T) (k:N) (P:T -> Prop) (f:N -> T -> bool),
+    contains T k P (al_filter f l) -> contains T k P l.
+Proof.
+  Hint Resolve <- contains_inv.
+  intros l k P f. induction l as [|[k' v] t IH].
+  - auto.
+  - simpl. destruct (f k' v) eqn:fkv.
+    + rewrite contains_inv. destruct 1 as [[ke Pv] | contains_filter_t]; auto.
+    + auto.
+Qed.
+
+Theorem al_filter_invariant :
+  forall (l:assoc_list T) (f:N -> T -> bool),
+    al_invariant T l -> al_invariant T (al_filter f l).
+Proof.
+  Hint Resolve al_filter_subset al_invariant_cons.
+  Hint Unfold in_domain.
+  intros l f H. induction l as [|[k v] t IH].
+  - auto.
+  - simpl. inversion H; subst. destruct (f k v) eqn:fkv; eauto 7.
+Qed.
+
+End Filter.
+
+Definition update {T:Type} (k:N) (f:T -> T) (l:assoc_list T) : assoc_list T :=
+  match assoc k l with
+    | None   => l
+    | Some v => insert k v l
+  end.
+
+Definition insert_merge {T:Type} (k:N) (f:T -> T) (def:T) (l:assoc_list T) : 
+  assoc_list T :=
+  insert k (f (match assoc k l with
+                 | None   => def
+                 | Some v => v
+               end)) l.
+
+Definition al_map {A B:Type} (f:N -> A -> B) : assoc_list A -> assoc_list B :=
+  map (fun x => match x with (k,v) => (k,f k v) end).
