MappingDB.v
@@ -1,0 +1,104 @@
+Require Import NArith.
+Require Import List.
+Require Import AssocList.
+
+Section MappingDB.
+
+Variable kernel_object : Type.
+
+Definition mapping_db : Type := assoc_list (assoc_list kernel_object).
+
+Definition has_mapping (pd:N) (sel:N) (ko:kernel_object) : mapping_db -> Prop :=
+  contains _ pd (contains _ sel (eq ko)).
+
+Definition create_mapping (pd:N) (sel:N) (ko:kernel_object) : mapping_db -> mapping_db :=
+  insert_merge pd (insert sel ko) empty.
+
+Definition remove_mapping (pd:N) (sel:N) : mapping_db -> mapping_db :=
+  update pd (remove sel).
+
+Fixpoint restrict (exceptions:assoc_list (list N)) : mapping_db -> mapping_db :=
+  al_map (fun pd mappings =>
+    match assoc pd exceptions with
+      | None     => mappings
+      | Some exc =>
+        al_filter (fun sel _ => if in_dec N.eq_dec sel exc then true else false) mappings
+    end).
+
+
+Definition remove_all (f:kernel_object -> bool) : mapping_db -> mapping_db :=
+  al_map (fun _ => al_filter (fun _ => f)).
+
+Definition remove_all_except
+           (f:kernel_object -> bool)
+           (exceptions:assoc_list (list N))
+           (db:mapping_db) : mapping_db :=
+  union (restrict exceptions db) (remove_all f db).
+
+Theorem create_preserve_other :
+  forall (db:mapping_db) (pd pd':N) (sel sel':N) (ko ko':kernel_object),
+    (pd' <> pd \/ sel' <> sel) -> al_invariant _ db ->
+    (has_mapping pd sel ko db
+     <-> has_mapping pd sel ko (create_mapping pd' sel' ko' db)).
+Proof.
+  Hint Resolve <- insert_preserve_other.
+  Hint Resolve contains_insert.
+  intros db pd pd' sel sel' ko ko' ineq inv_db. split.
+  - unfold create_mapping. unfold insert_merge. destruct (assoc pd' db) eqn:A.
+    + intros H. unfold has_mapping. destruct (N.eq_dec pd' pd); subst; eauto.
+      destruct ineq as [pde | sele].
+      * eauto.
+      * apply contains_insert. apply insert_preserve_other. assumption. unfold has_mapping in H. apply assoc_in_contains in A.
+        apply contains_combine with (P1 := eq a) in H.
+        unfold contains in H. destruct H as [v [in_db [av E]]].
+        unfold contains. subst. assumption. assumption. assumption.
+    + destruct (N.eq_dec pd' pd). 
+      * destruct ineq as [H|H]; try tauto. subst. unfold has_mapping. intros P. 
+        apply contains_in_domain in P. apply assoc_not_in in A. contradiction.
+      * intros. unfold has_mapping. apply insert_preserve_other. assumption.
+        assumption.
+  - unfold create_mapping. unfold insert_merge. intros H. unfold has_mapping.
+    destruct (assoc pd' db) eqn:A.
+    + destruct ineq as [ineq|ineq]. 
+      * apply insert_preserve_other in H; assumption.
+      * destruct (N.eq_dec pd' pd).
+        subst. unfold has_mapping in H.
+Abort.
+
+Theorem create_has_mapping :
+  forall (db:mapping_db) (pd:N) (sel:N) (ko:kernel_object),
+    has_mapping pd sel ko (create_mapping pd sel ko db).
+Proof.
+Abort.
+
+Theorem remove_removes_mapping :
+  forall (db:mapping_db) (pd:N) (sel:N) (ko:kernel_object),
+    ~has_mapping pd sel ko (remove_mapping pd sel db).
+Proof.
+Abort.
+
+Theorem remove_preserve_other :
+  forall (db:mapping_db) (pd pd':N) (sel sel':N) (ko:kernel_object),
+    (pd' <> pd /\ sel <> sel') ->
+    (has_mapping pd sel ko db <-> has_mapping pd sel ko (remove_mapping pd sel db)).
+Proof.
+Abort.
+
+Theorem remove_all_except_removes :
+  forall (db:mapping_db) (pd:N) (sel:N) (ko:kernel_object) (f:kernel_object -> bool)
+         (exceptions:assoc_list (list N)),
+    has_mapping pd sel ko (remove_all_except f exceptions db) ->
+    f ko = false \/ contains (list N) pd (In sel) exceptions.
+Proof.
+Abort.
+
+Theorem remove_all_except_preseve_other :
+  forall (db:mapping_db) (pd:N) (sel:N) (ko:kernel_object) (f:kernel_object -> bool)
+         (exceptions:assoc_list (list N)),
+    f ko = true ->
+    (has_mapping pd sel ko db <->
+     has_mapping pd sel ko (remove_all_except f exceptions db)).
+Proof.
+Abort.
+
+End MappingDB.
